

函数：f(z) = 1 / (1 + exp( − z))

导数：f(z)' = f(z)(1 − f(z))

```py
import tensorflow as tf

a = tf.constant([[1.0, 2.0], [1.0, 2.0], [1.0, 2.0]])
sess = tf.Session()
print(sess.run(tf.sigmoid(a)))
```
output:
[[ 0.7310586 0.88079703]
[ 0.7310586 0.88079703]
[ 0.7310586 0.88079703]]

```py
import tensorflow as tf

input_data = tf.Variable( [1,1,1] , dtype = tf.float32 )
output = tf.nn.sigmoid(input_data)
with tf.Session() as sess:
    init = tf.initialize_all_variables()
    sess.run(init)
    print(sess.run(output))
```
[0.7310586 0.7310586 0.7310586]

## 参考

1. https://blog.csdn.net/Eric_LH/article/details/79077962
2. https://www.cnblogs.com/lovephysics/p/7219169.html